\[
T(n) = 
\begin{cases} 
      \text{T(n-1)+n} & \text{; n > 1} \\
      \text{1} & \text{; n = 1}
\end{cases}
\]

T(n) = T(n-1) + n  //eq(1) //equation
T(n-1) = T(n-2) + (n-1)  //eq(2)
T(n-2) = T(n-3) + (n-2)  //eq(3)

eq(2) in eq(3) //substitute equation

T(n) = T(n-q) + n
T(n) = T(n-2) + (n-1) + n
T(n) = T(n-3) + (n-2) + (n-1) + n
.
.
.
If we keep substituting for some arbitary k
value, we eventually get

T(k) = T(n-k) + (n-k+1) + .... + (n-2) + (n-1) + n

// For what value of k does this become 1, T(n-k)

n - k = 1
k = n - 1

// Now substitute this k value
// In place of k, substitute the value n-1

= T(n-(n-1)) + (n-(n-1)+1) + ...(n+2) + (n-1) + n
= T(n-n+1) + (n-n+1+1) + ... + (n+2) + (n-1) + n
T(n) = T(1) + 2 + ... + (n-2) + (n-1) + n
= 1 + 2 + .... + (n+2) + (n-1) + n

// sum of first n natural numbers

T(n) = \(\frac{n(n+1)}{2}\)
=> O(n^2^)

// simplification example for O(n^2^)

T(n) = \(\frac{n(n+1)}{2}\)
= \(\frac{n^2+n}{2}\)
=> O(n^2^)

---


\[
T(n) = 
\begin{cases} 
      T(n-1) + n^2 & \text{if } n > 1 \\
      1 & \text{if } n = 1
\end{cases}
\]

n^k^ => O(n^k+1^)

---

// Find the \(k_th\) fibonacci number

```
fib(n)
  if n <= 1
    return n
  else
    return fib(n-1) + fib(n-2)
```
// recurrence relation

\[
T(n) = 
\begin{cases} 
      \text{T(n-1) + T(n-2) + 1} & \text{; n > 1} \\
      \text{1} & \text{; n <= 1}
\end{cases}
\]

T(n-1) is approximately T(n-2)
// The time take to compute the second fib number


\[
T(n) = 
\begin{cases} 
      \text{2T(n-1) + 1} & \text{; n > 1} \\
      \text{1} & \text{; n <= 1}
\end{cases}
\]

// use backwards substitution method
T(n) = 2T(n-1)+ 1 //eq1
T(n-1) = 2T(n-2) + 1 //eq2
T(n-2) = 2T(n-3) + 1 //eq3


//substitute for T(n-1)

T(n) = 2T(n-1) + 1
= 2[2T(n-2)+1] + 1
= 2^2^+T(n-2) + 2 + 1

// substitute the value 2T(n-2)+1 to get the value
// now substitute the value of T(n-2)
= 2^2^[2T(n-3)+1]+2+1
= 2^3^T(n-3)+4+2+1

// and if we keep doing this for some arbitary value k, then it's
// going to be 2 to the power of k

T(k) = 2^k^T(n-2)+2^k-1^+...2^2^+2+1

// From the start to the end

// alternatively

T(k) = 2^k^T(n-k) + 2^k^ - 1

// now we want to find the value that makes the T(n-k) one

n - k = 0
k = n

T(n) = 2^n^T(n-n)+2^n^-1

// now

= 2^n^(1) + 2^n^-1
=> T(n) = 2^n^ + 2^n^-1
=> O(2.2^n^ - 1)
=> O(2^n^)

---

// You can write any recursive problem iteratively

```
fib(n) {
  int fib = 0
  int a = 0
  for (int i = 0; i < n; i++)
    fib = fib + a
    a = fib
  return fib
}
```

=> O(n)

// This is going to be in the exam


---

// programming time

``` java

/*
1 int is 4 bytes
an array is better than just a bunch of ints
memory addresses are in hexadecimal
*/
import java.util.ArrayList;

public static int[] fillArray(int[] arr) {
    for(int i = 0; i < arr.length; i++)
        arr[i] = (int)(Math.random() * 100);
        return arr;
}

public static void printArray(int[] arr) {
    for(int i:arr)
        System.out.print(i + " ");
        System.out.println();
}

public static boolean equalArray(int[] arr1, int[] arr2) {
    if (arr1 == null || arr2 == null)
        return false;
    if(arr1.length != arr2.length)
        return false;
    for(int i = 0; i< arr1.length; i++)
        if(arr1[i] != arr2[i])
            return false
    return true;
}

public static int[] copyArray(int[] from, int[] to) {
    for(int i = 0; i < from.length; i++)
        to[i] = from[i];
    return to;
}

public class Main
{
	public static void main(String[] args) {
		
// 		ArrayList<Integer> nums = new ArrayList;
        int[] A = new int[5];
        int[] B = new int[5];
        
        System.out.println(A);
        System.out.println(B);
        A = fillArray(A);
        B = fillArray(B);
        
        printArray(A);
        printArray(B);
        
        System.out.println(A == B);
        B = A;
        System.out.println(A == B);
        printArray(A);
        printArray(B);
	}
}
```