The Fibonacci sequence is defined by the recurrence relation:

$$
F(n) = 
\begin{cases} 
      0 & \text{if } n = 0 \\
      1 & \text{if } n = 1 \\
      F(n-1) + F(n-2) & \text{if } n > 1
\end{cases}
$$


The general formula for the sequence is:

$$
a_n = f(n) \quad \text{for} \quad n = 1, 2, 3, \dots
$$


The first few terms of the sequence are:

- \( a_1 = 1 \)
- \( a_2 = 2 \)
- \( a_3 = 3 \)
- \( a_4 = 4 \)
- \( \dots \)


The sum of the first \( n \) terms of a sequence is:

$$
\sum_{n=1}^{N} a_n
$$


The closed-form formula for the sequence is:

$$
a_n = 3n + 1
$$


### Fibonacci Sequence Example:

The Fibonacci sequence is defined by the following recurrence relation:

$$
F(n) = 
\begin{cases} 
      0 & \text{if } n = 0 \\
      1 & \text{if } n = 1 \\
      F(n-1) + F(n-2) & \text{if } n > 1
\end{cases}
$$

### Arithmetic Sequence Example:

An arithmetic sequence with a common difference \( d \) is written as:

$$
a_n = a_1 + (n-1) \cdot d
$$

The sum of the first \( n \) terms is:

$$
S_n = \sum_{n=1}^{N} a_n
$$


\[
O(n), \quad \Omega(n), \quad \Theta(n), \quad \infty
\]

\[
a + b = c \quad \text{and} \quad x + y = z
\]
